compiler/backend/proofs/README.md
@@ -99,15 +99,8 @@ Correctness proof for lab_filter
 [lab_to_targetProofScript.sml](lab_to_targetProofScript.sml):
 Correctness proof for lab_to_target
 
-[source_rewriterProofsScript.sml](source_rewriterProofsScript.sml):
-Correctness proofs for the expression rewriting function
-Shows that matchesExpr e p = SOME s ==> appExpr p s = SOME e
-
 [source_to_flatProofScript.sml](source_to_flatProofScript.sml):
 Correctness proof for source_to_flat
-
-[source_to_sourceProofsScript.sml](source_to_sourceProofsScript.sml):
-Correctness proofs for floating-point optimizations
 
 [stack_allocProofScript.sml](stack_allocProofScript.sml):
 Correctness proof for stack_alloc
